rpartrec code

src/rpartrec.lean
@@ -4,536 +4,13 @@ import computability.partrec_code
 import computability.halting
 import data.pfun
 import tactic
+import code
 
 open encodable denumerable roption
 
-namespace nat.rpartrec
-
-inductive code : Type
-| oracle : code
-| zero   : code
-| succ   : code
-| left   : code
-| right  : code
-| pair   : code → code → code
-| comp   : code → code → code
-| prec   : code → code → code
-| rfind' : code → code
-| univn  : code → code
-
-end nat.rpartrec
-
-namespace nat.rpartrec.code
-open nat (mkpair unpair)
-open nat.rpartrec (code)
-
-protected def const : ℕ → code
-| 0     := zero
-| (n+1) := comp succ (const n)
-
-protected def id : code := pair left right
-
-def curry (c : code) (n : ℕ) : code :=
-comp c (pair (code.const n) code.id)
-
-def encode_code : code → ℕ
-| oracle       := 0
-| zero         := 1
-| succ         := 2
-| left         := 3
-| right        := 4
-| (pair cf cg) := (bit0 $ bit0 $ bit0 (mkpair (encode_code cf) (encode_code cg))) + 5
-| (comp cf cg) := (bit0 $ bit0 $ bit1 (mkpair (encode_code cf) (encode_code cg))) + 5
-| (prec cf cg) := (bit0 $ bit1 $ bit0 (mkpair (encode_code cf) (encode_code cg))) + 5
-| (rfind' cf)  := (bit0 $ bit1 $ bit1 (encode_code cf)) + 5
-| (univn cf)   := (bit1 (encode_code cf)) + 5
-
-lemma guygk (n) : n ≤ n+9 := nat.le.intro rfl
-
-def of_nat_code : ℕ → code
-| 0 := oracle
-| 1 := zero
-| 2 := succ
-| 3 := left
-| 4 := right
-| (e+5) :=
-  have div8 : e.div2.div2.div2 ≤ e :=
-    by { simp[nat.div2_val], 
-         exact le_trans (nat.div_le_self (e/2/2) 2) 
-         (le_trans (nat.div_le_self (e/2) 2) (nat.div_le_self e 2)) },
-  have e.div2.div2.div2 < e + 5 := nat.lt_succ_iff.mpr (le_trans div8 (nat.le.intro rfl)),
-  have e.div2.div2.div2.unpair.1 < e + 5 := nat.lt_succ_iff.mpr
-    (le_trans (le_trans (nat.unpair_le_left _) div8) (nat.le.intro rfl)),
-  have e.div2.div2.div2.unpair.2 < e + 5 := nat.lt_succ_iff.mpr
-    (le_trans (le_trans (nat.unpair_le_right _) div8) (nat.le.intro rfl)),
-  have e.div2 < e + 5 := nat.lt_succ_iff.mpr
-    (le_trans (by simp[nat.div2_val]; exact nat.div_le_self _ _) (nat.le.intro rfl)),
-  match e.bodd, e.div2.bodd, e.div2.div2.bodd with
-  | ff, ff, ff := pair (of_nat_code e.div2.div2.div2.unpair.1)
-                        (of_nat_code e.div2.div2.div2.unpair.2)
-  | ff, ff, tt := comp (of_nat_code e.div2.div2.div2.unpair.1)
-                        (of_nat_code e.div2.div2.div2.unpair.2)
-  | ff, tt, ff := prec (of_nat_code e.div2.div2.div2.unpair.1)
-                        (of_nat_code e.div2.div2.div2.unpair.2)
-  | ff, tt, tt := rfind' (of_nat_code e.div2.div2.div2)
-  | tt, _,  _  := univn (of_nat_code e.div2)
-end
-
-private lemma encode_of_nat_code : ∀ e, encode_code (of_nat_code e) = e
-| 0     := rfl
-| 1     := rfl
-| 2     := rfl
-| 3     := rfl
-| 4     := rfl
-| (e+5) :=
-  have div8 : e.div2.div2.div2 ≤ e :=
-    by { simp[nat.div2_val], 
-         exact le_trans (nat.div_le_self (e/2/2) 2) 
-         (le_trans (nat.div_le_self (e/2) 2) (nat.div_le_self e 2)) },
-  have e.div2.div2.div2 < e + 5 := nat.lt_succ_iff.mpr (le_trans div8 (nat.le.intro rfl)),
-  have e.div2.div2.div2.unpair.1 < e + 5 := nat.lt_succ_iff.mpr
-    (le_trans (le_trans (nat.unpair_le_left _) div8) (nat.le.intro rfl)),
-  have e.div2.div2.div2.unpair.2 < e + 5 := nat.lt_succ_iff.mpr
-    (le_trans (le_trans (nat.unpair_le_right _) div8) (nat.le.intro rfl)),
-  have e.div2 < e + 5 := nat.lt_succ_iff.mpr
-    (le_trans (by simp[nat.div2_val]; exact nat.div_le_self _ _) (nat.le.intro rfl)),
-  have IH : _ := encode_of_nat_code e.div2.div2.div2,
-  have IH1 : _ := encode_of_nat_code e.div2.div2.div2.unpair.1,
-  have IH2 : _ := encode_of_nat_code e.div2.div2.div2.unpair.2,
-  have IH3 : _ := encode_of_nat_code e.div2,
-  begin
-    suffices :
-      (of_nat_code (e + 5)).encode_code =
-      nat.bit e.bodd (nat.bit e.div2.bodd (nat.bit e.div2.div2.bodd e.div2.div2.div2)) + 5,
-    { simp[nat.bit_decomp, this] },
-    simp [encode_code, of_nat_code],
-    cases e.bodd; simp [encode_code, of_nat_code, nat.bit, IH, IH1, IH2],
-    cases e.div2.bodd; cases e.div2.div2.bodd;
-    simp [encode_code, of_nat_code, nat.bit, IH, IH1, IH2],
-    { have h : ∀ m : ℕ, cond m.bodd bit1 bit0 m.div2 = m,
-      { intros m, exact nat.bit_decomp m }, simp[h, IH3] }
-  end
-
-private lemma of_nat_code_encode : ∀ c, of_nat_code (encode_code c) = c
-| oracle       := rfl
-| zero         := rfl
-| succ         := rfl
-| left         := rfl
-| right        := rfl
-| (pair cf cg) := by { simp[encode_code, of_nat_code],
-    exact ⟨of_nat_code_encode cf, of_nat_code_encode cg⟩ }
-| (comp cf cg) := by { simp[encode_code, of_nat_code],
-    exact ⟨of_nat_code_encode cf, of_nat_code_encode cg⟩ }
-| (prec cf cg) := by { simp[encode_code, of_nat_code],
-    exact ⟨of_nat_code_encode cf, of_nat_code_encode cg⟩ }
-| (rfind' cf)  := by { simp[encode_code, of_nat_code],
-    exact of_nat_code_encode cf }
-| (univn cf)   := by { simp[encode_code, of_nat_code],
-    exact of_nat_code_encode cf }
-
-instance : denumerable code :=
-mk' ⟨encode_code, of_nat_code,
-  of_nat_code_encode,
-  encode_of_nat_code⟩
-
-def evaln : ℕ → (ℕ → option ℕ) → code → ℕ → option ℕ
-| 0     f _            := λ _, none
-| (s+1) f oracle       := λ n, guard (n ≤ s) >> f n
-| (k+1) f zero         := λ n, guard (n ≤ k) >> pure 0
-| (k+1) f succ         := λ n, guard (n ≤ k) >> pure (nat.succ n)
-| (k+1) f left         := λ n, guard (n ≤ k) >> pure n.unpair.1
-| (k+1) f right        := λ n, guard (n ≤ k) >> pure n.unpair.2
-| (s+1) f (pair cf cg) := λ n, guard (n ≤ s) >>
-    mkpair <$> evaln (s+1) f cf n <*> evaln (s+1) f cg n
-| (s+1) f (comp cf cg) := λ n, guard (n ≤ s) >>
-    do x ← evaln (s+1) f cg n, evaln (s+1) f cf x
-| (s+1) f (prec cf cg) := λ n, guard (n ≤ s) >>
-    n.unpaired (λ a n,
-    n.cases (evaln (s+1) f cf a) $ λ y, do
-    i ← evaln s f (prec cf cg) (mkpair a y),
-    evaln (s+1) f cg (mkpair a (mkpair y i)))
-| (s+1) f (rfind' cf)  := λ n, guard (n ≤ s) >>
-    n.unpaired (λ a m, do
-    x ← evaln (s+1) f cf (mkpair a m),
-    if x = 0 then pure m else
-    evaln s f (rfind' cf) (mkpair a (m+1)))
-| (s+1) f (univn cf)       := λ n, guard (n ≤ s) >> 
-    evaln (min s n.unpair.1.unpair.1)
-    (evaln (s+1) f cf) (of_nat _ n.unpair.1.unpair.2) n.unpair.2
-
-theorem evaln_univn {s f cf} :
-  evaln (s+1) f (univn cf) = (λ n, guard (n ≤ s) >> 
-  evaln n.unpair.1.unpair.1 (evaln (s+1) f cf) (of_nat _ n.unpair.1.unpair.2) n.unpair.2) :=
-funext $ λ n,
-by { have : n ≤ s ∨ ¬n ≤ s, exact em (n ≤ s), cases this;
-     simp[evaln, (>>), failure, alternative.failure, this],  
-     have : min s n.unpair.fst.unpair.fst = n.unpair.1.unpair.1,
-     { simp, exact le_trans (nat.unpair_le_left  _) (le_trans (nat.unpair_le_left _) this) },
-     rw this }
-
-theorem evaln_univn0 {s f cf} :
-  (λ n, guard (n ≤ s) >> 
-  evaln (min s n.unpair.1.unpair.1) (evaln (s+1) f cf) (of_nat _ n.unpair.1.unpair.2) n.unpair.2) =
-  (λ n, guard (n ≤ s) >> 
-  evaln n.unpair.1.unpair.1 (evaln (s+1) f cf) (of_nat _ n.unpair.1.unpair.2) n.unpair.2) :=
-funext $ λ n,
-by { have : n ≤ s ∨ ¬n ≤ s, exact em (n ≤ s), cases this;
-     simp[evaln, (>>), failure, alternative.failure, this], 
-     have : min s n.unpair.fst.unpair.fst = n.unpair.1.unpair.1,
-     { simp, exact le_trans (nat.unpair_le_left  _) (le_trans (nat.unpair_le_left _) this) },
-     rw this }
-
-theorem evaln_inclusion : ∀ {s c} {f g : ℕ → option ℕ},
-  (∀ x y, x < s → f x = some y → g x = some y) → 
-  ∀ x y, evaln s f c x = some y →  evaln s g c x = some y
-| 0 c _ _ := by simp[evaln]
-| (s+1) oracle f g := λ h n y, 
-    by { simp[evaln], have : n ≤ s ∨ ¬ n ≤ s, omega,
-         cases this; simp[(>>), this], exact h _ _ (nat.lt_succ_iff.mpr this),
-         intros _ c, exfalso, exact option.not_mem_none _ c }
-| (s+1) zero         f g := by simp[evaln]
-| (s+1) succ         f g := by simp[evaln]
-| (s+1) left         f g := by simp[evaln]
-| (s+1) right        f g := by simp[evaln]
-| (s+1) (pair cf cg) f g := λ h n y,
-    have IH0 : _ := @evaln_inclusion (s+1) cf _ _ h,
-    have IH1 : _ := @evaln_inclusion (s+1) cg _ _ h,
-    by { simp[evaln, (>>)], assume e hf,
-         have : ∃ y, evaln (s + 1) f cf n = some y, 
-         { cases evaln (s + 1) f cf n; simp, simp[(<*>), hf] at hf ⊢, exact hf },
-         rcases this with ⟨y0, hy0⟩, have IH0' := IH0 _ _ hy0,
-          have : ∃ y, evaln (s + 1) f cg n = some y, 
-         { cases evaln (s + 1) f cg n; simp, simp[(<*>), hf] at hf ⊢, exact hf },
-         rcases this with ⟨y1, hy1⟩, have IH1' := IH1 _ _ hy1,
-         simp[hy0, hy1, IH0', IH1'] at hf ⊢, exact ⟨e, hf⟩ }
-| (s+1) (comp cf cg) f g := λ h n y,
-    have IH0 : _ := @evaln_inclusion (s+1) cf _ _ h,
-    have IH1 : _ := @evaln_inclusion (s+1) cg _ _ h,
-    by { simp[evaln, (>>)], assume e z hz hy,
-         refine ⟨e, z, IH1 _ _ hz, IH0 _ _ hy⟩ }
-| (s+1) (prec cf cg) f g := λ h n y,
-    have l0 : ∀ x y, x < s → f x = some y → g x = some y :=
-      λ x y e, h x y (nat.lt.step e),
-    have IH0 : _ := @evaln_inclusion s (cf.prec cg) _ _ l0,
-    have IH1 : _ := @evaln_inclusion (s+1) cf _ _ h,
-    have IH2 : _ := @evaln_inclusion (s+1) cg _ _ h,
-    by { simp[evaln, (>>)], assume e hf,
-         cases n.unpair.snd with n0; simp at hf ⊢, exact ⟨e, IH1 _ _ hf⟩,
-         rcases hf with ⟨z, hz0, hz1⟩,
-         refine ⟨e, z, IH0 _ _ hz0, IH2 _ _ hz1⟩ }
-| (s+1) (rfind' cf)  f g := λ h n y, 
-    have l0 : ∀ x y, x < s → f x = some y → g x = some y :=
-      λ x y e, h x y (nat.lt.step e),
-    have IH0 : _ := @evaln_inclusion (s+1) cf _ _ h, 
-    have IH1 : _ := @evaln_inclusion s cf.rfind' _ _ l0,
-    by { simp[evaln, (>>)], assume e z ez ey,
-         refine ⟨e, z, IH0 _ _ ez, _⟩,
-         cases z with z0; simp at ey ⊢, exact ey, exact IH1 _ _ ey }
-| (s+1) (univn cf)  f g := λ h n y, 
-    have IH0 : _ := @evaln_inclusion (s+1) cf _ _ h,
-    have IH0 : _ := @evaln_inclusion
-      (min s n.unpair.fst.unpair.fst) (of_nat code n.unpair.fst.unpair.snd)
-      (evaln (s + 1) f cf) (evaln (s + 1) g cf) (λ x y _, IH0 x y),
-    by { simp[evaln, (>>)], assume e ey, refine ⟨e, IH0 _ _ ey⟩ }
-
-theorem evaln_use : ∀ {s c} {f g : ℕ → option ℕ},
-  (∀ x, x < s → f x = g x) → evaln s f c = evaln s g c
-| 0     c            _ _  := by simp[evaln]
-| (s+1) oracle       _ _  := λ h, funext $ λ n, 
-    by { simp[evaln], have : n ≤ s ∨ ¬ n ≤ s, omega,
-         cases this; simp[(>>), this], exact h _ (nat.lt_succ_iff.mpr this), refl }
-| (s+1) zero         f g := by simp[evaln]
-| (s+1) succ         f g := by simp[evaln]
-| (s+1) left         f g := by simp[evaln]
-| (s+1) right        f g := by simp[evaln]
-| (s+1) (pair cf cg) f g := λ h,
-    have IH0 : _ := @evaln_use (s+1) cf _ _ h,
-    have IH1 : _ := @evaln_use (s+1) cg _ _ h,
-    funext $ λ n, 
-    by { simp[evaln], have : n ≤ s ∨ ¬ n ≤ s, omega, cases this;
-         simp[(>>), this, IH0, IH1] }
-| (s+1) (comp cf cg) f g := λ h,
-    have IH0 : _ := @evaln_use (s+1) cf _ _ h,
-    have IH1 : _ := @evaln_use (s+1) cg _ _ h,
-    funext $ λ n, 
-    by { simp[evaln], have : n ≤ s ∨ ¬ n ≤ s, omega, cases this;
-         simp[(>>), this, IH0, IH1] }
-| (s+1) (prec cf cg) f g := λ h,
-    have l0 : ∀ (x : ℕ), x < s → f x = g x := λ x e, h x (nat.lt.step e),
-    have IH0 : _ := @evaln_use s (cf.prec cg) _ _ l0,
-    have IH1 : _ := @evaln_use (s+1) cf _ _ h,
-    have IH2 : _ := @evaln_use (s+1) cg _ _ h,
-    funext $ λ n, 
-    by { simp[evaln], have : n ≤ s ∨ ¬ n ≤ s, omega, cases this;
-         simp[(>>), this, IH0, IH1, IH2] }
-| (s+1) (rfind' cf)  f g := λ h, 
-    have l0 : ∀ (x : ℕ), x < s → f x = g x := λ x e, h x (nat.lt.step e),
-    have IH0 : _ := @evaln_use (s+1) cf _ _ h,
-    have IH1 : _ := @evaln_use s cf.rfind' _ _ l0,
-    funext $ λ n, 
-    by { simp[evaln], have : n ≤ s ∨ ¬ n ≤ s, omega, cases this;
-         simp[(>>), this, IH0, IH1] }
-| (s+1) (univn cf)   f g := λ h, funext $ λ n,
-    have IH0 : _ := @evaln_use (s+1) cf _ _ h,
-    have IH0 : _ := @evaln_use
-      (min s n.unpair.fst.unpair.fst) (of_nat code n.unpair.fst.unpair.snd)
-      (evaln (s + 1) f cf) (evaln (s + 1) g cf) (by simp[IH0]),
-    by { simp[evaln], have : n ≤ s ∨ ¬ n ≤ s, omega, cases this;
-         simp[(>>), this, IH0] }
-
-theorem evaln_use' {s} {f g : ℕ → option ℕ} (h : ∀ x, x < s → f x = g x) :
-  evaln s f = evaln s g := 
-funext $ λ c, evaln_use h
-
-def evaln_univn_oracle (f) (c : code) {s s' a : ℕ} (h : (s'.mkpair (encode c)).mkpair a < s) :
-  evaln s f (univn oracle) ((s'.mkpair (encode c)).mkpair a) = evaln s' f c a :=
-begin
-  suffices : evaln s f (univn oracle) ((s'.mkpair (encode c)).mkpair a) =
-  evaln s' (λ n, guard (n < s) >> f n) c a,
-  { rw this, 
-    have : ∀ x, x < s' → (λ n, guard (n < s) >> f n) x = f x,
-    { intros x ex, 
-      have : x < s := 
-      lt_trans (lt_of_lt_of_le ex (le_trans (nat.le_mkpair_left _ _) (nat.le_mkpair_left _ _))) h,
-      simp[(>>), this] },
-    have := evaln_use' this, simp[this] },
-  have e0 : s = (s - 1) + 1, omega, rw e0,
-  have e : min (s - 1) s' = s', simp,
-  { suffices : s' < s, omega,
-    exact lt_of_le_of_lt (le_trans (nat.le_mkpair_left _ _) (nat.le_mkpair_left _ _)) h },
-  have : (s'.mkpair (encode c)).mkpair a ≤ s - 1, omega,
-  simp[evaln, this, e, pure],
-  suffices : (λ (n : ℕ), guard (n ≤ s - 1) >> f n) =
-    (λ (n : ℕ), guard (n < s - 1 + 1) >> f n),
-  rw this, simp[this, (>>)], funext x, 
-  have : x ≤ s - 1 ↔ x < s - 1 + 1, from nat.lt_succ_iff.symm,
-  simp[this], congr,
-end
-
-theorem evaln_bound {f} : ∀ {k c n x}, x ∈ evaln k f c n → n < k
-| 0     c n x h := by simp [evaln] at h; cases h
-| (k+1) c n x h := begin
-  suffices : ∀ {o : option ℕ}, x ∈ guard (n ≤ k) >> o → n < k + 1,
-  { cases c; rw [evaln] at h; try { exact this h } },
-  simpa [(>>)] using nat.lt_succ_of_le
-end
-
-theorem evaln_mono : ∀ {s₁ s₂ c f n x},
-  s₁ ≤ s₂ → evaln s₁ f c n = some x → evaln s₂ f c n = some x
-| 0      _      _            _ _ _ := λ _ h, by simp [evaln] at h; cases h
-| (s₀+1) 0      _            _ _ _ := λ e h, by exfalso; exact nat.not_succ_le_zero s₀ e
-| (s₀+1) (s₁+1) oracle       f n x := λ hs,
-    by { simp[evaln], have : n ≤ s₀ ∨ ¬ n ≤ s₀, omega,
-         cases this; simp[(>>), this], exact λ e, ⟨by omega, e⟩,
-         intros _ c, exfalso, exact option.not_mem_none _ c }
-| (s₀+1) (s₁+1) zero         f n x := λ hs, 
-    by simp[evaln, (>>)]; exact λ _ e, ⟨by omega, e⟩
-| (s₀+1) (s₁+1) succ         f n x := λ hs, 
-    by simp[evaln, (>>)]; exact λ _ e, ⟨by omega, e⟩
-| (s₀+1) (s₁+1) left         f n x := λ hs, 
-    by simp[evaln, (>>)]; exact λ _ e, ⟨by omega, e⟩
-| (s₀+1) (s₁+1) right        f n x := λ hs, 
-    by simp[evaln, (>>)]; exact λ _ e, ⟨by omega, e⟩
-| (s₀+1) (s₁+1) (pair cf cg) f n x := λ hs,
-    have IH0 : _ := λ n y, @evaln_mono (s₀+1) (s₁+1) cf f n y hs,
-    have IH1 : _ := λ n y, @evaln_mono (s₀+1) (s₁+1) cg f n y hs,
-    by { simp[evaln, (>>)], assume e0 ex,
-         have : ∃ y, evaln (s₀ + 1) f cf n = some y,
-         { cases evaln (s₀ + 1) f cf n; simp[(<*>)] at ex ⊢, exact ex },
-         rcases this with ⟨y₀, hy₀⟩,
-         have : ∃ y, evaln (s₀ + 1) f cg n = some y,
-         { cases evaln (s₀ + 1) f cg n; simp[(<*>)] at ex ⊢, exact ex },         
-         rcases this with ⟨y₁, hy₁⟩,
-         simp[hy₀, hy₁, IH0 _ _ hy₀, IH1 _ _ hy₁] at ex ⊢,
-         exact ⟨le_trans e0 (nat.le_of_succ_le_succ hs), ex⟩ }
-| (s₀+1) (s₁+1) (comp cf cg) f n x := λ hs,        
-    have IH0 : _ := λ n y, @evaln_mono (s₀+1) (s₁+1) cf f n y hs,
-    have IH1 : _ := λ n y, @evaln_mono (s₀+1) (s₁+1) cg f n y hs,
-    by { simp[evaln, (>>)], assume e0 y ey ex,
-         refine ⟨le_trans e0 (nat.le_of_succ_le_succ hs), y, IH1 _ _ ey, IH0 _ _ ex⟩ }
-| (s₀+1) (s₁+1) (prec cf cg) f n x := λ hs,
-    have IH0 : _ := λ n y, @evaln_mono s₀ s₁ (cf.prec cg) f n y (nat.le_of_succ_le_succ hs),
-    have IH1 : _ := λ n y, @evaln_mono (s₀+1) (s₁+1) cf f n y hs,
-    have IH2 : _ := λ n y, @evaln_mono (s₀+1) (s₁+1) cg f n y hs,
-    by { simp[evaln, (>>)],
-         cases n.unpair.snd with n0; simp,
-         assume e0 ex,
-         exact ⟨le_trans e0 (nat.le_of_succ_le_succ hs), IH1 _ _ ex⟩,
-         assume e0 y ey ex,
-         refine ⟨le_trans e0 (nat.le_of_succ_le_succ hs), y, IH0 _ _ ey, IH2 _ _ ex⟩ }
-| (s₀+1) (s₁+1) (rfind' cf)  f n x := λ hs,
-    have IH0 : _ := λ n y, @evaln_mono (s₀+1) (s₁+1) cf f n y hs,
-    have IH1 : _ := λ n y, @evaln_mono s₀ s₁ cf.rfind' f n y (nat.le_of_succ_le_succ hs),
-    by { simp[evaln, (>>), pure],
-         assume e0 y ey ex,
-         refine ⟨by omega, y, IH0 _ _ ey, _⟩,
-         cases y with y0; simp at ex ⊢, exact ex, exact IH1 _ _ ex }
-| (s₀+1) (s₁+1) (univn cf)   f n x := λ hs,
-    have IH0 : _ := λ n y, @evaln_mono (s₀+1) (s₁+1) cf f n y hs,
-    have IH1 : _ := λ n y : ℕ, @evaln_mono
-      (min s₀ n.unpair.1.unpair.1) (min s₁ n.unpair.1.unpair.1)
-      (of_nat code n.unpair.fst.unpair.snd)
-      (evaln (s₀ + 1) f cf) n.unpair.2 y,
-    by { simp[evaln, (>>)], assume e ex,
-         have : min s₀ n.unpair.fst.unpair.fst ≤ min s₁ n.unpair.fst.unpair.fst :=
-         inf_le_inf_right _ (nat.le_of_succ_le_succ hs),
-         have := IH1 _ _ this ex, refine ⟨by omega, _⟩,
-         exact evaln_inclusion (λ x y _, IH0 x y) _ _ this }
-
-def eval (f : ℕ → option ℕ) : code → ℕ →. ℕ 
-| oracle := λ n, f n
-| zero         := pure 0
-| succ         := nat.succ
-| left         := ↑(λ n : ℕ, n.unpair.1)
-| right        := ↑(λ n : ℕ, n.unpair.2)
-| (pair cf cg) := λ n, mkpair <$> eval cf n <*> eval cg n
-| (comp cf cg) := λ n, eval cg n >>= eval cf
-| (prec cf cg) := nat.unpaired (λ a n,
-    n.elim (eval cf a) (λ y IH, do i ← IH, eval cg (mkpair a (mkpair y i))))
-| (rfind' cf) := nat.unpaired (λ a m,
-    (nat.rfind (λ n, (λ m, m = 0) <$>
-      eval cf (mkpair a (n + m)))).map (+ m))
-| (univn cf) := λ n, nat.rfind_opt
-    (λ s, guard (n ≤ s) >> evaln n.unpair.1.unpair.1 
-      (evaln (s+1) f cf) (of_nat _ n.unpair.1.unpair.2) n.unpair.2)
-
-lemma eval_univn_evaln_iff {f x n} {cf : code} :
-  x ∈ eval f cf.univn n ↔ (∃ k, evaln (k + 1) f cf.univn n = some x) :=
-begin
-  simp[eval, evaln_univn, (>>)],
-  let f := (λ s, guard (n ≤ s) >> evaln n.unpair.1.unpair.1
-    (evaln (s+1) f cf) (of_nat _ n.unpair.1.unpair.2) n.unpair.2),
-  have : ∀ a m n, m ≤ n → a ∈ f m → a ∈ f n,
-  { simp[f, (>>)], intros a s₀ s₁ e e0 ha, refine ⟨by omega, evaln_inclusion _ _ _ ha⟩, 
-    exact (λ x y _, evaln_mono (by omega)) },
-  have := (@nat.rfind_opt_mono _ _ this) x, simp [f, (>>)] at this, 
-  exact this
-end
-
-theorem evaln_sound {f} : ∀ {k c n x},
-  x ∈ evaln k f c n → x ∈ eval f c n
-| 0     _ n x h := by simp [evaln] at h; cases h
-| (k+1) c n x h := begin
-  induction c with cf cg hf hg cf cg hf hg cf cg hf hg cf hf cf hf generalizing x n;
-    simp [eval, evaln, (>>), (<*>)] at h ⊢, 
-  { exact h.2 },
-  { simp [pure, pfun.pure, eq_comm] at h ⊢, exact h.2 },
-  { simp [pure, pfun.pure, eq_comm] at h, exact h.2 },
-  { simp [pure, pfun.pure, eq_comm] at h, exact h.2 },
-  { simp [pure, pfun.pure, eq_comm] at h, exact h.2 },
-  { rcases h with ⟨_, y, ef, z, eg, rfl⟩,
-    exact ⟨_, hf _ _ ef, _, hg _ _ eg, rfl⟩ },
-  { rcases h with ⟨_, y, eg, ef⟩,
-    exact ⟨_, hg _ _ eg, hf _ _ ef⟩ },
-  { rcases h with ⟨_, h⟩,
-    revert h,
-    induction n.unpair.2 with m IH generalizing x; simp,
-    { apply hf },
-    { refine λ y h₁ h₂, ⟨y, IH _ _, _⟩,
-      { have := evaln_mono k.le_succ h₁,
-        simp [evaln, (>>)] at this,
-        exact this.2 },
-      { exact hg _ _ h₂ } } },
-  { rcases h with ⟨_, h⟩,
-    rcases h with ⟨m, h₁, h₂⟩,
-    by_cases m0 : m = 0; simp [m0] at h₂,
-    { exact ⟨0,
-       ⟨by simpa [m0] using hf _ _ h₁,
-        λ m, (nat.not_lt_zero _).elim⟩,
-        by injection h₂ with h₂; simp [h₂]⟩ },
-    { have := evaln_sound h₂, simp [eval] at this,
-      rcases this with ⟨y, ⟨hy₁, hy₂⟩, rfl⟩,
-      refine ⟨ y+1, ⟨by simpa [add_comm, add_left_comm] using hy₁, λ i im, _⟩,
-               by simp [add_comm, add_left_comm] ⟩,
-      cases i with i,
-      { exact ⟨m, by simpa using hf _ _ h₁, m0⟩ },
-      { rcases hy₂ (nat.lt_of_succ_lt_succ im) with ⟨z, hz, z0⟩,
-        exact ⟨z, by simpa [nat.succ_eq_add_one, add_comm, add_left_comm] using hz, z0⟩ } } },
-  { apply eval_univn_evaln_iff.mpr, use k, simp[evaln, (>>)], exact h },
-end
-
-theorem evaln_complete {f : ℕ → option ℕ} {c n x} :
-  x ∈ eval (λ x, f x) c n ↔ ∃ k, x ∈ evaln k f c n := ⟨λ h,
-begin
-  suffices : ∃ k, x ∈ evaln (k+1) f c n,
-  { exact let ⟨k, h⟩ := this in ⟨k+1, h⟩ },
-    induction c generalizing n x;
-    simp [eval, evaln, pure, pfun.pure, (<*>), (>>)] at h ⊢,
-    { exact ⟨⟨n, by refl⟩, h⟩ },
-    { use n, have : min n n.unpair.fst.unpair.fst = n.unpair.fst.unpair.fst,
-      { simp, exact le_trans (nat.unpair_le_left _) (nat.unpair_le_left _) }, simp [this,h] },
-    { exact ⟨⟨_, le_refl _⟩, h.symm⟩ },
-    { exact ⟨⟨_, le_refl _⟩, h.symm⟩ },
-    { exact ⟨⟨_, le_refl _⟩, h.symm⟩ },
-    case nat.rpartrec.code.pair : cf cg hf hg 
-    { rcases h with ⟨x, hx, y, hy, rfl⟩,
-      rcases hf hx with ⟨k₁, hk₁⟩, rcases hg hy with ⟨k₂, hk₂⟩,
-      refine ⟨max k₁ k₂, le_max_left_of_le $ nat.le_of_lt_succ $ evaln_bound hk₁, x, _, y, _, rfl⟩,
-      exact evaln_mono (nat.succ_le_succ $ le_max_left _ _) hk₁, 
-      exact evaln_mono (nat.succ_le_succ $ le_max_right _ _) hk₂ },
-    case nat.rpartrec.code.comp : cf cg hf hg 
-    { rcases h with ⟨y, hy, hx⟩,
-      rcases hf hx with ⟨k₁, hk₁⟩, rcases hg hy with ⟨k₂, hk₂⟩,
-      refine ⟨max k₂ k₁, le_max_left_of_le $ nat.le_of_lt_succ $ evaln_bound hk₂, y, _, _⟩,
-      exact evaln_mono (nat.succ_le_succ $ le_max_left _ _) hk₂,
-      exact evaln_mono (nat.succ_le_succ $ le_max_right _ _) hk₁ },
-    case nat.rpartrec.code.prec : cf cg hf hg
-    { revert h,
-      generalize : n.unpair.1 = n₁, generalize : n.unpair.2 = n₂,
-      induction n₂ with m IH generalizing x n; simp,
-      { intro, rcases hf h with ⟨k, hk⟩,
-        exact ⟨_, le_max_left _ _,
-          evaln_mono (nat.succ_le_succ $ le_max_right _ _) hk⟩ },
-      { intros y hy hx,
-        rcases IH hy with ⟨k₁, nk₁, hk₁⟩, rcases hg hx with ⟨k₂, hk₂⟩,
-        refine ⟨(max k₁ k₂).succ, nat.le_succ_of_le $ le_max_left_of_le $
-          le_trans (le_max_left _ (mkpair n₁ m)) nk₁, y,
-          evaln_mono (nat.succ_le_succ $ le_max_left _ _) _,
-          evaln_mono (nat.succ_le_succ $ nat.le_succ_of_le $ le_max_right _ _) hk₂⟩,
-        simp [evaln, (>>)],
-        exact ⟨le_trans (le_max_right _ _) nk₁, hk₁⟩ } },
-    case nat.rpartrec.code.rfind' : cf hf
-    { rcases h with ⟨y, ⟨hy₁, hy₂⟩, rfl⟩,
-      suffices : ∃ k, y + n.unpair.2 ∈ evaln (k+1) f (rfind' cf)
-        (mkpair n.unpair.1 n.unpair.2), {simpa [evaln, (>>)]},
-      revert hy₁ hy₂, generalize : n.unpair.2 = m, intros,
-      induction y with y IH generalizing m; simp [evaln, (>>)],
-      { simp at hy₁, rcases hf hy₁ with ⟨k, hk⟩,
-        exact ⟨_, nat.le_of_lt_succ $ evaln_bound hk, _, hk, by simp; refl⟩ },
-      { rcases hy₂ (nat.succ_pos _) with ⟨a, ha, a0⟩,
-        rcases hf ha with ⟨k₁, hk₁⟩,
-        rcases IH m.succ
-            (by simpa [nat.succ_eq_add_one, add_comm, add_left_comm] using hy₁)
-            (λ i hi, by simpa [nat.succ_eq_add_one, add_comm, add_left_comm] using
-              hy₂ (nat.succ_lt_succ hi))
-          with ⟨k₂, hk₂⟩,
-        use (max k₁ k₂).succ,
-        rw [zero_add] at hk₁,
-        use (nat.le_succ_of_le $ le_max_left_of_le $ nat.le_of_lt_succ $ evaln_bound hk₁),
-        use a,
-        use evaln_mono (nat.succ_le_succ $ nat.le_succ_of_le $ le_max_left _ _) hk₁,
-        simpa [nat.succ_eq_add_one, a0, -max_eq_left, -max_eq_right, add_comm, add_left_comm] using
-            evaln_mono (nat.succ_le_succ $ le_max_right _ _) hk₂ } },
-    case nat.rpartrec.code.univn : cf hf
-    { have := eval_univn_evaln_iff.mp h, simp[evaln, (>>)] at this, exact this }
-end, λ ⟨k, h⟩, evaln_sound h⟩
-
-@[simp] theorem eval_const (f) : ∀ n m, eval f (code.const n) m = roption.some n
-| 0     m := rfl
-| (n+1) m := by simp! *
-
-@[simp] theorem eval_id (f n) : eval f code.id n = roption.some n := by simp! [(<*>)]
-
-@[simp] theorem eval_curry (f c n x) : eval f (curry c n) x = eval f c (mkpair n x) :=
-by simp! [(<*>)]
-
-end nat.rpartrec.code
-
 namespace nat
 
-instance {α β} : has_coe (α → option β) (α →. β) := ⟨λ f, (λ x, f x)⟩
-
-inductive rpartrec (o : ℕ → option ℕ) : (ℕ →. ℕ) → Prop
+inductive rpartrec (o : ℕ →. ℕ) : (ℕ →. ℕ) → Prop
 | oracle : rpartrec (λ x, o x)
 | zero : rpartrec (pure 0)
 | succ : rpartrec succ
@@ -544,18 +21,18 @@ inductive rpartrec (o : ℕ → option ℕ) : (ℕ →. ℕ) → Prop
 | prec {f g} : rpartrec f → rpartrec g → rpartrec (unpaired (λ a n,
     n.elim (f a) (λ y IH, do i ← IH, g (mkpair a (mkpair y i)))))
 | rfind {f} : rpartrec f → rpartrec (λ a, rfind (λ n, (λ m, m = 0) <$> f (mkpair a n)))
-| univn {f : ℕ → option ℕ} : rpartrec f → rpartrec (unpaired $ λ a n, 
-    nat.rpartrec.code.evaln a.unpair.1 f (of_nat _ a.unpair.2) n)
+| univn {f : ℕ →. ℕ} [decidable_pred f.dom] : rpartrec f → rpartrec (unpaired $ λ a n, 
+    nat.rpartrec.code.evaln a.unpair.1 f.eval_opt (of_nat _ a.unpair.2) n)
 
 namespace rpartrec
 
 def reducible (f g) : Prop := rpartrec g f
-local infix ` pr_in `:80 := reducible
+local infix ` partrec_in `:80 := reducible
 
-theorem of_eq {o} {f g : ℕ →. ℕ} (hf : rpartrec o f) (H : ∀ n, f n = g n) : rpartrec o g :=
+theorem of_eq {o f g : ℕ →. ℕ} (hf : rpartrec o f) (H : ∀ n, f n = g n) : rpartrec o g :=
 (funext H : f = g) ▸ hf
 
-theorem of_partrec {f} (g) (hf : nat.partrec f) : f pr_in g :=
+theorem of_partrec {f} (g) (hf : nat.partrec f) : f partrec_in g :=
 begin
   induction hf,
   case nat.partrec.zero { exact zero },
@@ -568,49 +45,81 @@ begin
   case nat.partrec.rfind : f pf hf { exact rfind hf },
 end
 
-theorem of_primrec {f} (g) (hf : primrec f) : f pr_in g := 
+theorem of_primrec {f} (g) (hf : primrec f) : f partrec_in g := 
 of_partrec g (partrec.of_primrec hf)
 
-protected theorem some {f} : roption.some pr_in f := of_primrec f primrec.id
+protected theorem some {f} : roption.some partrec_in f := of_primrec f primrec.id
 
-theorem none {f} : (λ n, none) pr_in f := of_partrec f partrec.none
+theorem none {f} : (λ n, none) partrec_in f := of_partrec f partrec.none
 
-theorem prec' {f g h o} (hf : f pr_in o) (hg : g pr_in o) (hh : h pr_in o) :
-  (λ a, (f a).bind (λ n, n.elim (g a) (λ y IH, do i ← IH, h (mkpair a (mkpair y i))))) pr_in o :=
+theorem prec' {f g h o} (hf : f partrec_in o) (hg : g partrec_in o) (hh : h partrec_in o) :
+  (λ a, (f a).bind (λ n, n.elim (g a) (λ y IH, do i ← IH, h (mkpair a (mkpair y i))))) partrec_in o :=
 ((prec hg hh).comp (pair rpartrec.some hf)).of_eq $ λ a, ext $ λ s, by simp [(<*>)]
 
-theorem refl {f : ℕ → option ℕ} : f pr_in f := oracle
+theorem refl {f : ℕ →. ℕ} : f partrec_in f := oracle
 
-theorem trans {f g h : ℕ → option ℕ} : f pr_in g → g pr_in h → f pr_in h :=
+theorem trans {f g h : ℕ →. ℕ} : f partrec_in g → g partrec_in h → f partrec_in h :=
 begin
   assume pgf phg,
   induction pgf,
   case oracle { exact phg },
-  case univn : f hf pf { exact univn pf },
+  case univn : _ _ _ pf { exactI univn pf },
   case zero { exact zero },
   case succ { exact succ },
   case left { exact left },
   case right { exact right },
-  case pair : f g hf hg pf pg { exact pair pf pg },
-  case comp : f g hf hg pf pg { exact comp pf pg },
-  case prec : f g hf hg pf pg { exact prec pf pg },
-  case rfind : f pf hf { exact rfind hf },
+  case pair : _ _ _ _ pf pg { exact pair pf pg },
+  case comp : _ _ _ _ pf pg { exact comp pf pg },
+  case prec : _ _ _ _ pf pg { exact prec pf pg },
+  case rfind : _ _ pf { exact rfind pf },
 end
 
 end rpartrec
 
 end nat
-def pfun_opt  (α : Type*) (β : Type*) := α → option β
-infixr ` →o `:25 := pfun_opt
 
 def rpartrec {α β σ τ} [primcodable α] [primcodable β] [primcodable σ] [primcodable τ] 
-  (f : α →. σ) (g : β → option τ) := nat.rpartrec.reducible
+  (f : α →. σ) (g : β →. τ) := nat.rpartrec.reducible
 (λ n, roption.bind (decode α n) (λ a, (f a).map encode))
-(λ n, option.bind (decode β n) (λ a, (g a).map encode))
-infix ` pr_in `:80 := rpartrec
+(λ n, roption.bind (decode β n) (λ a, (g a).map encode))
+infix ` partrec_in `:80 := rpartrec
 
 def rcomputable {α β σ τ} [primcodable α] [primcodable β] [primcodable σ] [primcodable τ]
-  (f : α → σ) (g : β → option τ) := (f : α →. σ) pr_in g
+  (f : α → σ) (g : β →. τ) := (f : α →. σ) partrec_in g
 infix ` computable_in `:80 := rcomputable
 
+theorem partrec.to_rpart {α σ β τ} [primcodable α] [primcodable σ] [primcodable β] [primcodable τ]
+  {f : α →. σ} {g : β →. τ} (h : partrec f) : f partrec_in g := nat.rpartrec.of_partrec _ h
 
+theorem partrec.to_rpart_in {α σ β τ} [primcodable α] [primcodable σ] [primcodable β] [primcodable τ]
+  {f : α →. σ} (g : β →. τ) (h : partrec f) : f partrec_in g := nat.rpartrec.of_partrec _ h
+
+theorem computable.to_rcomp {α σ β τ} [primcodable α] [primcodable σ] [primcodable β] [primcodable τ]
+  {f : α → σ} {g : β →. τ} (h : computable f) : f computable_in g := nat.rpartrec.of_partrec _ h
+
+theorem computable.to_rcomp_in {α σ β τ} [primcodable α] [primcodable σ] [primcodable β] [primcodable τ]
+  {f : α → σ} (g : β →. τ) (h : computable f) : f computable_in g := nat.rpartrec.of_partrec _ h
+
+namespace rpartrec
+variables {α : Type*} {β : Type*} {γ : Type*} {σ : Type*} {τ : Type*} {μ : Type*}
+variables [primcodable α] [primcodable β] [primcodable γ] [primcodable σ] [primcodable τ] [primcodable μ]
+
+theorem of_eq {f g : α →. σ} {h : β →. τ} (hf : f partrec_in h) (H : ∀ n, f n = g n) : g partrec_in h :=
+(funext H : f = g) ▸ hf
+
+theorem comp {f : β →. γ} {g : α → β} {h : σ →. τ} 
+  (hf : f partrec_in h) (hg : (g : α →. β) partrec_in h) : (λ a, f (g a)) partrec_in h :=
+(nat.rpartrec.comp hf hg).of_eq $ λ n, by simp; cases e : decode α n with a; simp [e, encodek]
+
+theorem nat_elim {f : α → ℕ} {g : α →. σ} {h : α × ℕ × σ →. σ} {i : β →. γ}
+  (hf : (f : α →. ℕ) partrec_in i) (hg : g partrec_in i) (hh : h partrec_in i) :
+  (λ a, (f a).elim (g a) (λ y IH, IH.bind (λ i, h (a, y, i)))) partrec_in i :=
+(nat.rpartrec.prec' hf hg hh).of_eq $ λ n, begin
+  cases e : decode α n with a; simp [e],
+  induction f a with m IH; simp,
+  rw [IH, bind_map],
+  congr, funext s,
+  simp [encodek]
+end
+
+end rpartrec
