src/code.lean
@@ -1,0 +1,544 @@
+import computability.partrec
+import computability.partrec_code
+import data.pfun
+import tactic
+
+open encodable denumerable roption
+
+namespace nat.rpartrec
+
+inductive code : Type
+| oracle : code
+| zero   : code
+| succ   : code
+| left   : code
+| right  : code
+| pair   : code → code → code
+| comp   : code → code → code
+| prec   : code → code → code
+| rfind' : code → code
+| univn  : code → code
+
+end nat.rpartrec
+
+namespace nat.rpartrec.code
+open nat (mkpair unpair)
+open nat.rpartrec (code)
+
+protected def const : ℕ → code
+| 0     := zero
+| (n+1) := comp succ (const n)
+
+protected def id : code := pair left right
+
+def curry (c : code) (n : ℕ) : code :=
+comp c (pair (code.const n) code.id)
+
+def encode_code : code → ℕ
+| oracle       := 0
+| zero         := 1
+| succ         := 2
+| left         := 3
+| right        := 4
+| (pair cf cg) := (bit0 $ bit0 $ bit0 (mkpair (encode_code cf) (encode_code cg))) + 5
+| (comp cf cg) := (bit0 $ bit0 $ bit1 (mkpair (encode_code cf) (encode_code cg))) + 5
+| (prec cf cg) := (bit0 $ bit1 $ bit0 (mkpair (encode_code cf) (encode_code cg))) + 5
+| (rfind' cf)  := (bit0 $ bit1 $ bit1 (encode_code cf)) + 5
+| (univn cf)   := (bit1 (encode_code cf)) + 5
+
+lemma guygk (n) : n ≤ n+9 := nat.le.intro rfl
+
+def of_nat_code : ℕ → code
+| 0 := oracle
+| 1 := zero
+| 2 := succ
+| 3 := left
+| 4 := right
+| (e+5) :=
+  have div8 : e.div2.div2.div2 ≤ e :=
+    by { simp[nat.div2_val], 
+         exact le_trans (nat.div_le_self (e/2/2) 2) 
+         (le_trans (nat.div_le_self (e/2) 2) (nat.div_le_self e 2)) },
+  have e.div2.div2.div2 < e + 5 := nat.lt_succ_iff.mpr (le_trans div8 (nat.le.intro rfl)),
+  have e.div2.div2.div2.unpair.1 < e + 5 := nat.lt_succ_iff.mpr
+    (le_trans (le_trans (nat.unpair_le_left _) div8) (nat.le.intro rfl)),
+  have e.div2.div2.div2.unpair.2 < e + 5 := nat.lt_succ_iff.mpr
+    (le_trans (le_trans (nat.unpair_le_right _) div8) (nat.le.intro rfl)),
+  have e.div2 < e + 5 := nat.lt_succ_iff.mpr
+    (le_trans (by simp[nat.div2_val]; exact nat.div_le_self _ _) (nat.le.intro rfl)),
+  match e.bodd, e.div2.bodd, e.div2.div2.bodd with
+  | ff, ff, ff := pair (of_nat_code e.div2.div2.div2.unpair.1)
+                        (of_nat_code e.div2.div2.div2.unpair.2)
+  | ff, ff, tt := comp (of_nat_code e.div2.div2.div2.unpair.1)
+                        (of_nat_code e.div2.div2.div2.unpair.2)
+  | ff, tt, ff := prec (of_nat_code e.div2.div2.div2.unpair.1)
+                        (of_nat_code e.div2.div2.div2.unpair.2)
+  | ff, tt, tt := rfind' (of_nat_code e.div2.div2.div2)
+  | tt, _,  _  := univn (of_nat_code e.div2)
+end
+
+private lemma encode_of_nat_code : ∀ e, encode_code (of_nat_code e) = e
+| 0     := rfl
+| 1     := rfl
+| 2     := rfl
+| 3     := rfl
+| 4     := rfl
+| (e+5) :=
+  have div8 : e.div2.div2.div2 ≤ e :=
+    by { simp[nat.div2_val], 
+         exact le_trans (nat.div_le_self (e/2/2) 2) 
+         (le_trans (nat.div_le_self (e/2) 2) (nat.div_le_self e 2)) },
+  have e.div2.div2.div2 < e + 5 := nat.lt_succ_iff.mpr (le_trans div8 (nat.le.intro rfl)),
+  have e.div2.div2.div2.unpair.1 < e + 5 := nat.lt_succ_iff.mpr
+    (le_trans (le_trans (nat.unpair_le_left _) div8) (nat.le.intro rfl)),
+  have e.div2.div2.div2.unpair.2 < e + 5 := nat.lt_succ_iff.mpr
+    (le_trans (le_trans (nat.unpair_le_right _) div8) (nat.le.intro rfl)),
+  have e.div2 < e + 5 := nat.lt_succ_iff.mpr
+    (le_trans (by simp[nat.div2_val]; exact nat.div_le_self _ _) (nat.le.intro rfl)),
+  have IH₀ : _ := encode_of_nat_code e.div2.div2.div2,
+  have IH₁ : _ := encode_of_nat_code e.div2.div2.div2.unpair.1,
+  have IH₂ : _ := encode_of_nat_code e.div2.div2.div2.unpair.2,
+  have IH₃ : _ := encode_of_nat_code e.div2,
+  begin
+    suffices :
+      (of_nat_code (e + 5)).encode_code =
+      nat.bit e.bodd (nat.bit e.div2.bodd (nat.bit e.div2.div2.bodd e.div2.div2.div2)) + 5,
+    { simp[nat.bit_decomp, this] },
+    simp [encode_code, of_nat_code],
+    cases e.bodd; simp [encode_code, of_nat_code, nat.bit, IH₀, IH₁, IH₂],
+    cases e.div2.bodd; cases e.div2.div2.bodd;
+    simp [encode_code, of_nat_code, nat.bit, IH₀, IH₁, IH₂],
+    { have h : ∀ m : ℕ, cond m.bodd bit1 bit0 m.div2 = m,
+      { intros m, exact nat.bit_decomp m }, simp[h, IH₃] }
+  end
+
+private lemma of_nat_code_encode : ∀ c, of_nat_code (encode_code c) = c
+| oracle       := rfl
+| zero         := rfl
+| succ         := rfl
+| left         := rfl
+| right        := rfl
+| (pair cf cg) := by { simp[encode_code, of_nat_code],
+    exact ⟨of_nat_code_encode cf, of_nat_code_encode cg⟩ }
+| (comp cf cg) := by { simp[encode_code, of_nat_code],
+    exact ⟨of_nat_code_encode cf, of_nat_code_encode cg⟩ }
+| (prec cf cg) := by { simp[encode_code, of_nat_code],
+    exact ⟨of_nat_code_encode cf, of_nat_code_encode cg⟩ }
+| (rfind' cf)  := by { simp[encode_code, of_nat_code],
+    exact of_nat_code_encode cf }
+| (univn cf)   := by { simp[encode_code, of_nat_code],
+    exact of_nat_code_encode cf }
+
+instance : denumerable code :=
+mk' ⟨encode_code, of_nat_code,
+  of_nat_code_encode,
+  encode_of_nat_code⟩
+
+def evaln : ℕ → (ℕ → option ℕ) → code → ℕ → option ℕ
+| 0     f _            := λ _, none
+| (s+1) f oracle       := λ n, guard (n ≤ s) >> f n
+| (s+1) f zero         := λ n, guard (n ≤ s) >> pure 0
+| (s+1) f succ         := λ n, guard (n ≤ s) >> pure (nat.succ n)
+| (s+1) f left         := λ n, guard (n ≤ s) >> pure n.unpair.1
+| (s+1) f right        := λ n, guard (n ≤ s) >> pure n.unpair.2
+| (s+1) f (pair cf cg) := λ n, guard (n ≤ s) >>
+    mkpair <$> evaln (s+1) f cf n <*> evaln (s+1) f cg n
+| (s+1) f (comp cf cg) := λ n, guard (n ≤ s) >>
+    do x ← evaln (s+1) f cg n, evaln (s+1) f cf x
+| (s+1) f (prec cf cg) := λ n, guard (n ≤ s) >>
+    n.unpaired (λ a n,
+    n.cases (evaln (s+1) f cf a) $ λ y, do
+    i ← evaln s f (prec cf cg) (mkpair a y),
+    evaln (s+1) f cg (mkpair a (mkpair y i)))
+| (s+1) f (rfind' cf)  := λ n, guard (n ≤ s) >>
+    n.unpaired (λ a m, do
+    x ← evaln (s+1) f cf (mkpair a m),
+    if x = 0 then pure m else
+    evaln s f (rfind' cf) (mkpair a (m+1)))
+| (s+1) f (univn cf)       := λ n, guard (n ≤ s) >> 
+    evaln (min s n.unpair.1.unpair.1)
+    (evaln (s+1) f cf) (of_nat _ n.unpair.1.unpair.2) n.unpair.2
+
+def evaln_ropt (s : ℕ) (f : ℕ →. ℕ) [decidable_pred f.dom] : code → ℕ → option ℕ :=
+evaln s f.eval_opt
+
+theorem evaln_univn {s f cf} :
+  evaln (s+1) f (univn cf) = (λ n, guard (n ≤ s) >> 
+  evaln n.unpair.1.unpair.1 (evaln (s+1) f cf) (of_nat _ n.unpair.1.unpair.2) n.unpair.2) :=
+funext $ λ n,
+by { have : n ≤ s ∨ ¬n ≤ s, exact em (n ≤ s), cases this;
+     simp[evaln, (>>), failure, alternative.failure, this],  
+     have : min s n.unpair.fst.unpair.fst = n.unpair.1.unpair.1,
+     { simp, exact le_trans (nat.unpair_le_left  _) (le_trans (nat.unpair_le_left _) this) },
+     rw this }
+
+theorem evaln_univn0 {s f cf} :
+  (λ n, guard (n ≤ s) >> 
+  evaln (min s n.unpair.1.unpair.1) (evaln (s+1) f cf) (of_nat _ n.unpair.1.unpair.2) n.unpair.2) =
+  (λ n, guard (n ≤ s) >> 
+  evaln n.unpair.1.unpair.1 (evaln (s+1) f cf) (of_nat _ n.unpair.1.unpair.2) n.unpair.2) :=
+funext $ λ n,
+by { have : n ≤ s ∨ ¬n ≤ s, exact em (n ≤ s), cases this;
+     simp[evaln, (>>), failure, alternative.failure, this], 
+     have : min s n.unpair.fst.unpair.fst = n.unpair.1.unpair.1,
+     { simp, exact le_trans (nat.unpair_le_left  _) (le_trans (nat.unpair_le_left _) this) },
+     rw this }
+
+theorem evaln_inclusion : ∀ {s c} {f g : ℕ → option ℕ},
+  (∀ x y, x < s → f x = some y → g x = some y) → 
+  ∀ x y, evaln s f c x = some y →  evaln s g c x = some y
+| 0 c _ _ := by simp[evaln]
+| (s+1) oracle f g := λ h n y, 
+    by { simp[evaln], have : n ≤ s ∨ ¬ n ≤ s, omega,
+         cases this; simp[(>>), this], exact h _ _ (nat.lt_succ_iff.mpr this),
+         intros _ c, exfalso, exact option.not_mem_none _ c }
+| (s+1) zero         f g := by simp[evaln]
+| (s+1) succ         f g := by simp[evaln]
+| (s+1) left         f g := by simp[evaln]
+| (s+1) right        f g := by simp[evaln]
+| (s+1) (pair cf cg) f g := λ h n y,
+    have IH₀ : _ := @evaln_inclusion (s+1) cf _ _ h,
+    have IH₁ : _ := @evaln_inclusion (s+1) cg _ _ h,
+    by { simp[evaln, (>>)], assume e hf,
+         have : ∃ y, evaln (s + 1) f cf n = some y, 
+         { cases evaln (s + 1) f cf n; simp, simp[(<*>), hf] at hf ⊢, exact hf },
+         rcases this with ⟨y0, hy0⟩, have IH₀' := IH₀ _ _ hy0,
+          have : ∃ y, evaln (s + 1) f cg n = some y, 
+         { cases evaln (s + 1) f cg n; simp, simp[(<*>), hf] at hf ⊢, exact hf },
+         rcases this with ⟨y1, hy1⟩, have IH₁' := IH₁ _ _ hy1,
+         simp[hy0, hy1, IH₀', IH₁'] at hf ⊢, exact ⟨e, hf⟩ }
+| (s+1) (comp cf cg) f g := λ h n y,
+    have IH₀ : _ := @evaln_inclusion (s+1) cf _ _ h,
+    have IH₁ : _ := @evaln_inclusion (s+1) cg _ _ h,
+    by { simp[evaln, (>>)], assume e z hz hy,
+         refine ⟨e, z, IH₁ _ _ hz, IH₀ _ _ hy⟩ }
+| (s+1) (prec cf cg) f g := λ h n y,
+    have l0 : ∀ x y, x < s → f x = some y → g x = some y :=
+      λ x y e, h x y (nat.lt.step e),
+    have IH₀ : _ := @evaln_inclusion s (cf.prec cg) _ _ l0,
+    have IH₁ : _ := @evaln_inclusion (s+1) cf _ _ h,
+    have IH₂ : _ := @evaln_inclusion (s+1) cg _ _ h,
+    by { simp[evaln, (>>)], assume e hf,
+         cases n.unpair.snd with n0; simp at hf ⊢, exact ⟨e, IH₁ _ _ hf⟩,
+         rcases hf with ⟨z, hz0, hz1⟩,
+         refine ⟨e, z, IH₀ _ _ hz0, IH₂ _ _ hz1⟩ }
+| (s+1) (rfind' cf)  f g := λ h n y, 
+    have l0 : ∀ x y, x < s → f x = some y → g x = some y :=
+      λ x y e, h x y (nat.lt.step e),
+    have IH₀ : _ := @evaln_inclusion (s+1) cf _ _ h, 
+    have IH₁ : _ := @evaln_inclusion s cf.rfind' _ _ l0,
+    by { simp[evaln, (>>)], assume e z ez ey,
+         refine ⟨e, z, IH₀ _ _ ez, _⟩,
+         cases z with z0; simp at ey ⊢, exact ey, exact IH₁ _ _ ey }
+| (s+1) (univn cf)  f g := λ h n y, 
+    have IH₀ : _ := @evaln_inclusion (s+1) cf _ _ h,
+    have IH₀ : _ := @evaln_inclusion
+      (min s n.unpair.fst.unpair.fst) (of_nat code n.unpair.fst.unpair.snd)
+      (evaln (s + 1) f cf) (evaln (s + 1) g cf) (λ x y _, IH₀ x y),
+    by { simp[evaln, (>>)], assume e ey, refine ⟨e, IH₀ _ _ ey⟩ }
+
+theorem evaln_use : ∀ {s c} {f g : ℕ → option ℕ},
+  (∀ x, x < s → f x = g x) → evaln s f c = evaln s g c
+| 0     c            _ _  := by simp[evaln]
+| (s+1) oracle       _ _  := λ h, funext $ λ n, 
+    by { simp[evaln], have : n ≤ s ∨ ¬ n ≤ s, omega,
+         cases this; simp[(>>), this], exact h _ (nat.lt_succ_iff.mpr this), refl }
+| (s+1) zero         f g := by simp[evaln]
+| (s+1) succ         f g := by simp[evaln]
+| (s+1) left         f g := by simp[evaln]
+| (s+1) right        f g := by simp[evaln]
+| (s+1) (pair cf cg) f g := λ h,
+    have IH₀ : _ := @evaln_use (s+1) cf _ _ h,
+    have IH₁ : _ := @evaln_use (s+1) cg _ _ h,
+    funext $ λ n, 
+    by { simp[evaln], have : n ≤ s ∨ ¬ n ≤ s, omega, cases this;
+         simp[(>>), this, IH₀, IH₁] }
+| (s+1) (comp cf cg) f g := λ h,
+    have IH₀ : _ := @evaln_use (s+1) cf _ _ h,
+    have IH₁ : _ := @evaln_use (s+1) cg _ _ h,
+    funext $ λ n, 
+    by { simp[evaln], have : n ≤ s ∨ ¬ n ≤ s, omega, cases this;
+         simp[(>>), this, IH₀, IH₁] }
+| (s+1) (prec cf cg) f g := λ h,
+    have l0 : ∀ (x : ℕ), x < s → f x = g x := λ x e, h x (nat.lt.step e),
+    have IH₀ : _ := @evaln_use s (cf.prec cg) _ _ l0,
+    have IH₁ : _ := @evaln_use (s+1) cf _ _ h,
+    have IH₂ : _ := @evaln_use (s+1) cg _ _ h,
+    funext $ λ n, 
+    by { simp[evaln], have : n ≤ s ∨ ¬ n ≤ s, omega, cases this;
+         simp[(>>), this, IH₀, IH₁, IH₂] }
+| (s+1) (rfind' cf)  f g := λ h, 
+    have l0 : ∀ (x : ℕ), x < s → f x = g x := λ x e, h x (nat.lt.step e),
+    have IH₀ : _ := @evaln_use (s+1) cf _ _ h,
+    have IH₁ : _ := @evaln_use s cf.rfind' _ _ l0,
+    funext $ λ n, 
+    by { simp[evaln], have : n ≤ s ∨ ¬ n ≤ s, omega, cases this;
+         simp[(>>), this, IH₀, IH₁] }
+| (s+1) (univn cf)   f g := λ h, funext $ λ n,
+    have IH₀ : _ := @evaln_use (s+1) cf _ _ h,
+    have IH₀ : _ := @evaln_use
+      (min s n.unpair.fst.unpair.fst) (of_nat code n.unpair.fst.unpair.snd)
+      (evaln (s + 1) f cf) (evaln (s + 1) g cf) (by simp[IH₀]),
+    by { simp[evaln], have : n ≤ s ∨ ¬ n ≤ s, omega, cases this;
+         simp[(>>), this, IH₀] }
+
+theorem evaln_use' {s} {f g : ℕ → option ℕ} (h : ∀ x, x < s → f x = g x) :
+  evaln s f = evaln s g := 
+funext $ λ c, evaln_use h
+
+def evaln_univn_oracle (f) (c : code) {s s' a : ℕ} (h : (s'.mkpair (encode c)).mkpair a < s) :
+  evaln s f (univn oracle) ((s'.mkpair (encode c)).mkpair a) = evaln s' f c a :=
+begin
+  suffices : evaln s f (univn oracle) ((s'.mkpair (encode c)).mkpair a) =
+  evaln s' (λ n, guard (n < s) >> f n) c a,
+  { rw this, 
+    have : ∀ x, x < s' → (λ n, guard (n < s) >> f n) x = f x,
+    { intros x ex, 
+      have : x < s := 
+      lt_trans (lt_of_lt_of_le ex (le_trans (nat.le_mkpair_left _ _) (nat.le_mkpair_left _ _))) h,
+      simp[(>>), this] },
+    have := evaln_use' this, simp[this] },
+  have e0 : s = (s - 1) + 1, omega, rw e0,
+  have e : min (s - 1) s' = s', simp,
+  { suffices : s' < s, omega,
+    exact lt_of_le_of_lt (le_trans (nat.le_mkpair_left _ _) (nat.le_mkpair_left _ _)) h },
+  have : (s'.mkpair (encode c)).mkpair a ≤ s - 1, omega,
+  simp[evaln, this, e, pure],
+  suffices : (λ (n : ℕ), guard (n ≤ s - 1) >> f n) =
+    (λ (n : ℕ), guard (n < s - 1 + 1) >> f n),
+  rw this, simp[this, (>>)], funext x, 
+  have : x ≤ s - 1 ↔ x < s - 1 + 1, from nat.lt_succ_iff.symm,
+  simp[this], congr,
+end
+
+theorem evaln_bound {f} : ∀ {k c n x}, x ∈ evaln k f c n → n < k
+| 0     c n x h := by simp [evaln] at h; cases h
+| (k+1) c n x h := begin
+  suffices : ∀ {o : option ℕ}, x ∈ guard (n ≤ k) >> o → n < k + 1,
+  { cases c; rw [evaln] at h; try { exact this h } },
+  simpa [(>>)] using nat.lt_succ_of_le
+end
+
+theorem evaln_mono : ∀ {s₁ s₂ c f n x},
+  s₁ ≤ s₂ → evaln s₁ f c n = some x → evaln s₂ f c n = some x
+| 0      _      _            _ _ _ := λ _ h, by simp [evaln] at h; cases h
+| (s₀+1) 0      _            _ _ _ := λ e h, by exfalso; exact nat.not_succ_le_zero s₀ e
+| (s₀+1) (s₁+1) oracle       f n x := λ hs,
+    by { simp[evaln], have : n ≤ s₀ ∨ ¬ n ≤ s₀, omega,
+         cases this; simp[(>>), this], exact λ e, ⟨by omega, e⟩,
+         intros _ c, exfalso, exact option.not_mem_none _ c }
+| (s₀+1) (s₁+1) zero         f n x := λ hs, 
+    by simp[evaln, (>>)]; exact λ _ e, ⟨by omega, e⟩
+| (s₀+1) (s₁+1) succ         f n x := λ hs, 
+    by simp[evaln, (>>)]; exact λ _ e, ⟨by omega, e⟩
+| (s₀+1) (s₁+1) left         f n x := λ hs, 
+    by simp[evaln, (>>)]; exact λ _ e, ⟨by omega, e⟩
+| (s₀+1) (s₁+1) right        f n x := λ hs, 
+    by simp[evaln, (>>)]; exact λ _ e, ⟨by omega, e⟩
+| (s₀+1) (s₁+1) (pair cf cg) f n x := λ hs,
+    have IH₀ : _ := λ n y, @evaln_mono (s₀+1) (s₁+1) cf f n y hs,
+    have IH₁ : _ := λ n y, @evaln_mono (s₀+1) (s₁+1) cg f n y hs,
+    by { simp[evaln, (>>)], assume e0 ex,
+         have : ∃ y, evaln (s₀ + 1) f cf n = some y,
+         { cases evaln (s₀ + 1) f cf n; simp[(<*>)] at ex ⊢, exact ex },
+         rcases this with ⟨y₀, hy₀⟩,
+         have : ∃ y, evaln (s₀ + 1) f cg n = some y,
+         { cases evaln (s₀ + 1) f cg n; simp[(<*>)] at ex ⊢, exact ex },         
+         rcases this with ⟨y₁, hy₁⟩,
+         simp[hy₀, hy₁, IH₀ _ _ hy₀, IH₁ _ _ hy₁] at ex ⊢,
+         exact ⟨le_trans e0 (nat.le_of_succ_le_succ hs), ex⟩ }
+| (s₀+1) (s₁+1) (comp cf cg) f n x := λ hs,        
+    have IH₀ : _ := λ n y, @evaln_mono (s₀+1) (s₁+1) cf f n y hs,
+    have IH₁ : _ := λ n y, @evaln_mono (s₀+1) (s₁+1) cg f n y hs,
+    by { simp[evaln, (>>)], assume e0 y ey ex,
+         refine ⟨le_trans e0 (nat.le_of_succ_le_succ hs), y, IH₁ _ _ ey, IH₀ _ _ ex⟩ }
+| (s₀+1) (s₁+1) (prec cf cg) f n x := λ hs,
+    have IH₀ : _ := λ n y, @evaln_mono s₀ s₁ (cf.prec cg) f n y (nat.le_of_succ_le_succ hs),
+    have IH₁ : _ := λ n y, @evaln_mono (s₀+1) (s₁+1) cf f n y hs,
+    have IH₂ : _ := λ n y, @evaln_mono (s₀+1) (s₁+1) cg f n y hs,
+    by { simp[evaln, (>>)],
+         cases n.unpair.snd with n0; simp,
+         assume e0 ex,
+         exact ⟨le_trans e0 (nat.le_of_succ_le_succ hs), IH₁ _ _ ex⟩,
+         assume e0 y ey ex,
+         refine ⟨le_trans e0 (nat.le_of_succ_le_succ hs), y, IH₀ _ _ ey, IH₂ _ _ ex⟩ }
+| (s₀+1) (s₁+1) (rfind' cf)  f n x := λ hs,
+    have IH₀ : _ := λ n y, @evaln_mono (s₀+1) (s₁+1) cf f n y hs,
+    have IH₁ : _ := λ n y, @evaln_mono s₀ s₁ cf.rfind' f n y (nat.le_of_succ_le_succ hs),
+    by { simp[evaln, (>>), pure],
+         assume e0 y ey ex,
+         refine ⟨by omega, y, IH₀ _ _ ey, _⟩,
+         cases y with y0; simp at ex ⊢, exact ex, exact IH₁ _ _ ex }
+| (s₀+1) (s₁+1) (univn cf)   f n x := λ hs,
+    have IH₀ : _ := λ n y, @evaln_mono (s₀+1) (s₁+1) cf f n y hs,
+    have IH₁ : _ := λ n y : ℕ, @evaln_mono
+      (min s₀ n.unpair.1.unpair.1) (min s₁ n.unpair.1.unpair.1)
+      (of_nat code n.unpair.fst.unpair.snd)
+      (evaln (s₀ + 1) f cf) n.unpair.2 y,
+    by { simp[evaln, (>>)], assume e ex,
+         have : min s₀ n.unpair.fst.unpair.fst ≤ min s₁ n.unpair.fst.unpair.fst :=
+         inf_le_inf_right _ (nat.le_of_succ_le_succ hs),
+         have := IH₁ _ _ this ex, refine ⟨by omega, _⟩,
+         exact evaln_inclusion (λ x y _, IH₀ x y) _ _ this }
+
+def eval (f : ℕ → option ℕ) : code → ℕ →. ℕ 
+| oracle := λ n, f n
+| zero         := pure 0
+| succ         := nat.succ
+| left         := ↑(λ n : ℕ, n.unpair.1)
+| right        := ↑(λ n : ℕ, n.unpair.2)
+| (pair cf cg) := λ n, mkpair <$> eval cf n <*> eval cg n
+| (comp cf cg) := λ n, eval cg n >>= eval cf
+| (prec cf cg) := nat.unpaired (λ a n,
+    n.elim (eval cf a) (λ y IH, do i ← IH, eval cg (mkpair a (mkpair y i))))
+| (rfind' cf) := nat.unpaired (λ a m,
+    (nat.rfind (λ n, (λ m, m = 0) <$>
+      eval cf (mkpair a (n + m)))).map (+ m))
+| (univn cf) := λ n, nat.rfind_opt
+    (λ s, guard (n ≤ s) >> evaln n.unpair.1.unpair.1 
+      (evaln (s+1) f cf) (of_nat _ n.unpair.1.unpair.2) n.unpair.2)
+
+lemma eval_univn_evaln_iff {f x n} {cf : code} :
+  x ∈ eval f cf.univn n ↔ (∃ k, evaln (k + 1) f cf.univn n = some x) :=
+begin
+  simp[eval, evaln_univn, (>>)],
+  let f := (λ s, guard (n ≤ s) >> evaln n.unpair.1.unpair.1
+    (evaln (s+1) f cf) (of_nat _ n.unpair.1.unpair.2) n.unpair.2),
+  have : ∀ a m n, m ≤ n → a ∈ f m → a ∈ f n,
+  { simp[f, (>>)], intros a s₀ s₁ e e0 ha, refine ⟨by omega, evaln_inclusion _ _ _ ha⟩, 
+    exact (λ x y _, evaln_mono (by omega)) },
+  have := (@nat.rfind_opt_mono _ _ this) x, simp [f, (>>)] at this, 
+  exact this
+end
+
+theorem evaln_sound {f} : ∀ {s c n x},
+  x ∈ evaln s f c n → x ∈ eval f c n
+| 0     _ _ _ h := by simp [evaln] at h; cases h
+| (s + 1) oracle n x h := by { simp [eval, evaln, (>>)] at h ⊢, exact h.2 }
+| (s + 1) zero   n x h := 
+    by { simp [eval, evaln, (>>), pure, pfun.pure] at h ⊢, exact eq.symm h.2 }
+| (s + 1) succ   n x h := 
+    by { simp [eval, evaln, (>>), pure, pfun.pure] at h ⊢, exact eq.symm h.2 }
+| (s + 1) left   n x h := 
+    by { simp [eval, evaln, (>>), pure, pfun.pure] at h ⊢, exact eq.symm h.2 }
+| (s + 1) right   n x h := 
+    by { simp [eval, evaln, (>>), pure, pfun.pure] at h ⊢, exact eq.symm h.2 }
+| (s + 1) (pair cf cg) n x h :=
+    have IH₀ : _ := @evaln_sound (s + 1) cf,
+    have IH₁ : _ := @evaln_sound (s + 1) cg,
+    by{ simp [eval, evaln, (>>), (<*>)] at h ⊢, 
+        rcases h with ⟨_, y, hy, z, hz, ex⟩,
+        refine ⟨y, IH₀ hy, z, IH₁ hz, ex⟩ }
+| (s + 1) (comp cf cg) n x h :=
+    have IH₀ : _ := @evaln_sound (s + 1) cf,
+    have IH₁ : _ := @evaln_sound (s + 1) cg,
+    by{ simp [eval, evaln, (>>), (<*>)] at h ⊢, 
+        rcases h with ⟨_, y, hy, hz⟩,
+        refine ⟨y, IH₁ hy, IH₀ hz⟩ }
+| (s + 1) (prec cf cg) n x h :=
+    have IH₀ : _ := @evaln_sound (s + 1) cf,
+    have IH₁ : _ := @evaln_sound (s + 1) cg,
+    by{ simp [eval, evaln, (>>)] at h ⊢,
+        rcases h with ⟨_, hx⟩, revert hx,
+        induction n.unpair.2 with m IH generalizing x; simp,
+        { exact IH₀ },
+        { refine λ y h₁ h₂, ⟨y, IH _ _, _⟩,
+          { have := evaln_mono s.le_succ h₁,
+        simp [evaln, (>>)] at this,
+        exact this.2 },
+        { exact IH₁ h₂ } } }
+| (s + 1) (rfind' cf) n x h :=
+    have IH₀ : _ := @evaln_sound (s+1) cf,
+    have IH₁ : _ := @evaln_sound s cf.rfind',
+  begin
+    simp [eval, evaln, (>>)] at h ⊢,
+    rcases h with ⟨_, m, hm, h⟩,
+    cases e : m with m0; simp[e, pure] at hm h,
+    { refine ⟨0, ⟨by simp; exact IH₀ hm, by simp⟩, by simp[h]⟩ },
+    { have := IH₁ h,  simp[eval] at this,
+      rcases this with ⟨y, ⟨hc0, hc1⟩, ex⟩,
+      refine ⟨y+1, ⟨
+        by simpa [add_comm, add_left_comm] using hc0, λ b eb, _⟩, 
+        by simpa [add_comm, add_left_comm] using ex⟩,
+      { cases b with b0, refine ⟨m0 + 1, by simp; exact IH₀ hm, by simp⟩, 
+        have : b0.succ + n.unpair.snd = b0 + (n.unpair.snd + 1), omega,
+        rw this, exact hc1 (nat.lt_of_succ_lt_succ eb) } }
+  end
+| (s + 1) (univn cf) n x h := eval_univn_evaln_iff.mpr ⟨s, h⟩
+
+theorem evaln_complete {f : ℕ → option ℕ} {c n x} :
+  x ∈ eval (λ x, f x) c n ↔ ∃ k, x ∈ evaln k f c n := ⟨λ h,
+begin
+  suffices : ∃ k, x ∈ evaln (k+1) f c n,
+  { exact let ⟨k, h⟩ := this in ⟨k+1, h⟩ },
+    induction c generalizing n x;
+    simp [eval, evaln, pure, pfun.pure, (<*>), (>>)] at h ⊢,
+    { exact ⟨⟨n, by refl⟩, h⟩ },
+    { use n, have : min n n.unpair.fst.unpair.fst = n.unpair.fst.unpair.fst,
+      { simp, exact le_trans (nat.unpair_le_left _) (nat.unpair_le_left _) }, simp [this,h] },
+    { exact ⟨⟨_, le_refl _⟩, h.symm⟩ },
+    { exact ⟨⟨_, le_refl _⟩, h.symm⟩ },
+    { exact ⟨⟨_, le_refl _⟩, h.symm⟩ },
+    case nat.rpartrec.code.pair : cf cg hf hg 
+    { rcases h with ⟨x, hx, y, hy, rfl⟩,
+      rcases hf hx with ⟨k₁, hk₁⟩, rcases hg hy with ⟨k₂, hk₂⟩,
+      refine ⟨max k₁ k₂, le_max_left_of_le $ nat.le_of_lt_succ $ evaln_bound hk₁, x, _, y, _, rfl⟩,
+      exact evaln_mono (nat.succ_le_succ $ le_max_left _ _) hk₁, 
+      exact evaln_mono (nat.succ_le_succ $ le_max_right _ _) hk₂ },
+    case nat.rpartrec.code.comp : cf cg hf hg 
+    { rcases h with ⟨y, hy, hx⟩,
+      rcases hf hx with ⟨k₁, hk₁⟩, rcases hg hy with ⟨k₂, hk₂⟩,
+      refine ⟨max k₂ k₁, le_max_left_of_le $ nat.le_of_lt_succ $ evaln_bound hk₂, y, _, _⟩,
+      exact evaln_mono (nat.succ_le_succ $ le_max_left _ _) hk₂,
+      exact evaln_mono (nat.succ_le_succ $ le_max_right _ _) hk₁ },
+    case nat.rpartrec.code.prec : cf cg hf hg
+    { revert h,
+      generalize : n.unpair.1 = n₁, generalize : n.unpair.2 = n₂,
+      induction n₂ with m IH generalizing x n; simp,
+      { intro, rcases hf h with ⟨k, hk⟩,
+        exact ⟨_, le_max_left _ _,
+          evaln_mono (nat.succ_le_succ $ le_max_right _ _) hk⟩ },
+      { intros y hy hx,
+        rcases IH hy with ⟨k₁, nk₁, hk₁⟩, rcases hg hx with ⟨k₂, hk₂⟩,
+        refine ⟨(max k₁ k₂).succ, nat.le_succ_of_le $ le_max_left_of_le $
+          le_trans (le_max_left _ (mkpair n₁ m)) nk₁, y,
+          evaln_mono (nat.succ_le_succ $ le_max_left _ _) _,
+          evaln_mono (nat.succ_le_succ $ nat.le_succ_of_le $ le_max_right _ _) hk₂⟩,
+        simp [evaln, (>>)],
+        exact ⟨le_trans (le_max_right _ _) nk₁, hk₁⟩ } },
+    case nat.rpartrec.code.rfind' : cf hf
+    { rcases h with ⟨y, ⟨hy₁, hy₂⟩, rfl⟩,
+      suffices : ∃ k, y + n.unpair.2 ∈ evaln (k+1) f (rfind' cf)
+        (mkpair n.unpair.1 n.unpair.2), {simpa [evaln, (>>)]},
+      revert hy₁ hy₂, generalize : n.unpair.2 = m, intros,
+      induction y with y IH generalizing m; simp [evaln, (>>)],
+      { simp at hy₁, rcases hf hy₁ with ⟨k, hk⟩,
+        exact ⟨_, nat.le_of_lt_succ $ evaln_bound hk, _, hk, by simp; refl⟩ },
+      { rcases hy₂ (nat.succ_pos _) with ⟨a, ha, a0⟩,
+        rcases hf ha with ⟨k₁, hk₁⟩,
+        rcases IH m.succ
+            (by simpa [nat.succ_eq_add_one, add_comm, add_left_comm] using hy₁)
+            (λ i hi, by simpa [nat.succ_eq_add_one, add_comm, add_left_comm] using
+              hy₂ (nat.succ_lt_succ hi))
+          with ⟨k₂, hk₂⟩,
+        use (max k₁ k₂).succ,
+        rw [zero_add] at hk₁,
+        use (nat.le_succ_of_le $ le_max_left_of_le $ nat.le_of_lt_succ $ evaln_bound hk₁),
+        use a,
+        use evaln_mono (nat.succ_le_succ $ nat.le_succ_of_le $ le_max_left _ _) hk₁,
+        simpa [nat.succ_eq_add_one, a0, -max_eq_left, -max_eq_right, add_comm, add_left_comm] using
+            evaln_mono (nat.succ_le_succ $ le_max_right _ _) hk₂ } },
+    case nat.rpartrec.code.univn : cf hf
+    { have := eval_univn_evaln_iff.mp h, simp[evaln, (>>)] at this, exact this }
+end, λ ⟨k, h⟩, evaln_sound h⟩
+
+@[simp] theorem eval_const (f) : ∀ n m, eval f (code.const n) m = roption.some n
+| 0     m := rfl
+| (n+1) m := by simp! *
+
+@[simp] theorem eval_id (f n) : eval f code.id n = roption.some n := by simp! [(<*>)]
+
+@[simp] theorem eval_curry (f c n x) : eval f (curry c n) x = eval f c (mkpair n x) :=
+by simp! [(<*>)]
+
+end nat.rpartrec.code
